PAC_Checker/IICF_Copying_List.thy
@@ -1,0 +1,303 @@
+theory IICF_Copying_List
+  imports Isabelle_LLVM.IICF
+    Isabelle_LLVM.Proto_EOArray
+    Isabelle_LLVM.LLVM_DS_Open_List
+begin
+
+text \<open>This Theory defines a "copying list".
+  By copying list we mean that the list can hold impure objects,
+  for operations that take ownership of an object (i.e. @{term hd}),
+  we implement a destructive variant (that will destroy the list)
+  and a non-destructive variant that will copy the element and keep
+  the list intact. Container elements need to have an implementation of copy.\<close>
+
+section \<open>Basic Setup\<close>
+text \<open>Based on @{theory \<open>Isabelle_LLVM.LLVM_DS_Open_List\<close>}\<close>
+
+type_synonym 'a cl_list = \<open>'a node ptr\<close>
+
+(* Owning list segment *)
+definition \<open>olseg A xs p s \<equiv> EXS xsi. lseg xsi p s ** \<upharpoonleft>(list_assn (mk_assn A)) xs xsi\<close> 
+
+(* Owning list assertion *)
+definition \<open>cl_assn A \<equiv> mk_assn (\<lambda>xs p. olseg A xs p null)\<close>
+definition \<open>cl_assn' A \<equiv> \<upharpoonleft>(cl_assn A)\<close>
+ 
+lemma cl_assn_simps:
+  \<open>cl_assn' A [] p = \<up>(p=null)\<close>
+  \<open>cl_assn' A xs null = \<up>(xs=[])\<close>
+  \<open>cl_assn' A (x#xs) p = (EXS c q. \<upharpoonleft>ll_bpto (Node c q) p ** A x c ** cl_assn' A xs q)\<close>
+  unfolding cl_assn'_def cl_assn_def olseg_def
+  subgoal by (auto simp: sep_algebra_simps)
+  subgoal by (auto simp: sep_algebra_simps)
+  subgoal
+    apply (auto simp: sep_algebra_simps list_assn_cons1_conv)
+    (* Sledgehammer finds this - TODO: make nicer *)
+    proof -
+    { fix bb :: 'b and pp :: "'b node ptr" and bbs :: "'b list" and aa :: llvm_amemory and bba :: 'b and ppa :: "'b node ptr" and bbsa :: "'b list"
+      have "\<not> (\<upharpoonleft>ll_bpto (Node bb pp) p \<and>* A x bb \<and>* lseg bbs pp null \<and>* \<upharpoonleft>(list_assn (mk_assn A)) xs bbs) aa \<and> \<not> (\<upharpoonleft>ll_bpto (Node bba ppa) p \<and>* lseg bbsa ppa null \<and>* A x bba \<and>* \<upharpoonleft>(list_assn (mk_assn A)) xs bbsa) aa \<or> (\<exists>b pa bs ba pb bsa. (\<upharpoonleft>ll_bpto (Node b pa) p \<and>* A x b \<and>* lseg bs pa null \<and>* \<upharpoonleft>(list_assn (mk_assn A)) xs bs) aa \<and> (\<upharpoonleft>ll_bpto (Node ba pb) p \<and>* lseg bsa pb null \<and>* A x ba \<and>* \<upharpoonleft>(list_assn (mk_assn A)) xs bsa) aa)"
+     by (smt (verit) sep.mult.left_commute) }
+    then show "(\<lambda>a. \<exists>b bs pa. (\<upharpoonleft>ll_bpto (Node b pa) p \<and>* lseg bs pa null \<and>* A x b \<and>* \<upharpoonleft>(list_assn (mk_assn A)) xs bs) a) = (\<lambda>a. \<exists>b pa bs. (\<upharpoonleft>ll_bpto (Node b pa) p \<and>* A x b \<and>* lseg bs pa null \<and>* \<upharpoonleft>(list_assn (mk_assn A)) xs bs) a)"
+      by meson
+    qed
+  done 
+
+section \<open>non-destructive, non-copying operations\<close>
+text \<open>The following operations can be defined without having to decide
+  between a destructive and a non-destructive variant\<close>
+
+definition cl_empty :: \<open>_ cl_list llM\<close> where [llvm_code, llvm_inline]:
+  \<open>cl_empty \<equiv> Mreturn null\<close>
+
+lemma os_empty_rule[vcg_rules]: \<open>llvm_htriple \<box> cl_empty (\<lambda>r. cl_assn' A [] r)\<close>
+  unfolding cl_empty_def cl_assn'_def cl_assn_def olseg_def
+  by vcg
+
+lemma cl_empty_hnr[sepref_fr_rules]:
+  \<open>(uncurry0 cl_empty, uncurry0 (RETURN op_list_empty)) \<in> unit_assn\<^sup>k \<rightarrow>\<^sub>a (cl_assn' A)\<close>
+  by (sepref_to_hoare; vcg)
+
+definition cl_prepend :: \<open>'a::llvm_rep \<Rightarrow> 'a cl_list \<Rightarrow> 'a cl_list llM\<close> where [llvm_code, llvm_inline]:
+  \<open>cl_prepend x p = ll_ref (Node x p)\<close>
+
+lemma cl_prepend_rule[vcg_rules]:
+  \<open>llvm_htriple (cl_assn' A xs p ** A x xi) (cl_prepend xi p) (\<lambda>r. cl_assn' A (x # xs) r)\<close>
+  unfolding cl_prepend_def
+  supply [simp] = cl_assn_simps
+  by vcg
+
+lemma cl_prepend_hnr[sepref_fr_rules]:
+  \<open>(uncurry cl_prepend, uncurry (RETURN oo op_list_prepend))
+  \<in> A\<^sup>d *\<^sub>a (cl_assn' A)\<^sup>d \<rightarrow>\<^sub>a (cl_assn' A) \<close>
+  by (sepref_to_hoare; vcg)
+
+definition cl_length :: \<open>'a::llvm_rep cl_list \<Rightarrow> 'b::len2 word llM\<close> where [llvm_code]:
+  \<open>cl_length p \<equiv> doM{
+    (_, i) \<leftarrow> llc_while
+      (\<lambda>(p, _). ll_cmp (p \<noteq> null))
+      (\<lambda>(p, i). doM {
+        n \<leftarrow> ll_load p;
+        i \<leftarrow> ll_add i (signed_nat 1);
+        Mreturn (node.next n, i) 
+      }) (p, signed_nat 0);
+    Mreturn i 
+  }\<close>
+
+lemma to_bool_from_bool[simp]: \<open>to_bool (from_bool \<phi> :: 1 word) = \<phi>\<close>
+  by (cases \<phi>) (auto simp: from_bool_def)
+
+context begin
+interpretation llvm_prim_arith_setup .
+
+lemma ll_ptrcmp_ne_null_simp:
+  \<open>ll_ptrcmp_ne a null = doM { Mreturn (from_bool (a \<noteq> null))}\<close>
+  by (vcg_normalize; simp add: eq_commute[of null])
+
+lemma ll_ptrcmp_ne_null_rule[vcg_rules]:
+  \<open>llvm_htriple \<box> (ll_ptrcmp_ne a null) (\<lambda>r. \<upharpoonleft>bool.assn (a \<noteq> null) r)\<close>
+  unfolding ll_ptrcmp_ne_null_simp
+  supply [simp] = bool.assn_def
+  by vcg
+
+end
+
+lemma lseg_singleton: \<open>lseg [x] p q = \<upharpoonleft>ll_bpto (Node x q) p\<close>
+  by (simp add: sep_algebra_simps)
+
+lemma lseg_snoc: \<open>lseg ys p q ** \<upharpoonleft>ll_bpto (Node x r) q \<turnstile> lseg (ys@[x]) p r\<close>
+  by (metis lseg_fuse lseg_singleton)
+
+lemma lseg_pure_partD:
+  \<open>pure_part (lseg l p s) \<Longrightarrow> l = [] \<longrightarrow> p = s\<close>
+  by (cases l) auto
+
+context begin
+
+private lemma take_snoc:
+  \<open>i < length xs \<Longrightarrow> take (Suc i) xs = take i xs @ [xs ! i]\<close>
+  by (rule take_Suc_conv_app_nth)
+
+private lemma take_snoc':
+  \<open>i < length xs \<Longrightarrow> take (i + 1) xs = take i xs @ [xs ! i]\<close>
+  by (simp add: take_Suc_conv_app_nth)
+
+private lemma drop_plus1: \<open>drop (i + 1) xs = drop (Suc i) xs\<close>
+  by simp
+
+private lemma drop_head:
+  \<open>i < length xs \<Longrightarrow> drop i xs = xs ! i # drop (Suc i) xs\<close>
+  by (simp add: Cons_nth_drop_Suc)
+
+private lemma cl_length_step_entails:
+  assumes \<open>x < length xs\<close> \<open>\<flat>\<^sub>psnat.assn (Suc x) rc\<close>
+  shows \<open>ENTAILS
+    (\<upharpoonleft>ll_bpto (Node (xs ! x) xa) a ** lseg (drop (Suc x) xs) xa null ** lseg (take x xs) p a)
+    (EXS xb. (EXS x'. \<upharpoonleft>snat.assn x' rc ** lseg (take x' xs) p xa ** lseg (drop x' xs) xa null
+        ** \<up>(x' \<le> length xs \<and> (x' < length xs \<or> xa = null)) ** \<up>\<^sub>!(xb = length xs - x'))
+      ** \<up>\<^sub>d((xb, length xs - x) \<in> measure id) ** \<box>)\<close>
+proof -
+  have R: \<open>(\<upharpoonleft>ll_bpto (Node (xs ! x) xa) a ** lseg (drop (Suc x) xs) xa null
+      ** lseg (take x xs) p a)
+    = ((lseg (take x xs) p a ** \<upharpoonleft>ll_bpto (Node (xs ! x) xa) a)
+      ** lseg (drop (Suc x) xs) xa null)\<close>
+    by (simp add: sep_conj_aci)
+  have S: \<open>lseg (take x xs) p a ** \<upharpoonleft>ll_bpto (Node (xs ! x) xa) a
+      \<turnstile> lseg (take (Suc x) xs) p xa\<close>
+    using lseg_snoc[of \<open>take x xs\<close> p a \<open>xs ! x\<close> xa]
+    by (simp add: take_snoc[OF assms(1)])
+  have SP: \<open>\<upharpoonleft>ll_bpto (Node (xs ! x) xa) a ** lseg (drop (Suc x) xs) xa null
+      ** lseg (take x xs) p a
+    \<turnstile> lseg (take (Suc x) xs) p xa ** lseg (drop (Suc x) xs) xa null\<close>
+    unfolding R by (rule conj_entails_mono[OF S entails_refl])
+  show ?thesis
+    unfolding ENTAILS_def
+    apply (rule entails_pureI)
+    apply (rule entails_trans[OF SP])
+    apply (simp add: sep_conj_exists sep_algebra_simps)
+    apply (rule entails_exI[where x=\<open>length xs - Suc x\<close>])
+    apply (rule entails_exI[where x=\<open>Suc x\<close>])
+    using assms
+    by (auto simp: vcg_tag_defs extract_pure_assn snat.assn_pure
+      sep_algebra_simps pred_lift_extract_simps entails_def
+      dest!: pure_part_split_conj dest: lseg_pure_partD)
+qed
+
+lemma cl_length_spine_rule[vcg_rules]:
+  \<open>length xs < max_snat LENGTH('l) \<Longrightarrow> llvm_htriple
+    (\<upharpoonleft>os_list_assn xs p)
+    (cl_length p :: 'l::len2 word llM)
+    (\<lambda>n. \<upharpoonleft>snat.assn (length xs) n ** \<upharpoonleft>os_list_assn xs p)\<close>
+  unfolding cl_length_def
+  apply (rewrite annotate_llc_while [where
+    I = \<open>\<lambda>(p', ii) t. EXS i. \<upharpoonleft>snat.assn i ii
+                 ** lseg (take i xs) p p'
+                 ** lseg (drop i xs) p' null
+                 ** \<up>(i \<le> length xs \<and> (i < length xs \<or> p' = null))
+                 ** \<up>\<^sub>!(t = length xs - i)\<close>
+    and R = \<open>measure id\<close>])
+  supply [simp] = os_list_assn_def drop_head take_snoc take_snoc' drop_plus1
+    lseg_append lseg_singleton sep_conj_exists
+  apply vcg_monadify
+  apply vcg'
+  subgoal by (rule cl_length_step_entails; assumption)
+  subgoal for asf r a b x ra sa
+    apply (rule impI)
+    apply hypsubst
+    apply vcg'
+    done
+  by (tactic \<open>Defer_Slot.remove_slot_tac\<close>)
+
+end
+
+text \<open>Composing the spine rule with the element ownership: decompose \<open>cl_assn'\<close> into
+  the plain spine plus element-wise \<open>list_assn\<close> ownership (cf. \<open>ol_assn_os_conv\<close> in
+  \<open>IICF_Owning_List\<close>), then sandwich the framed spine rule. Plain \<open>vcg\<close> on such
+  decomposed triples reliably diverges, hence the manual composition via
+  \<open>htriple_pre_EXS\<close>/\<open>htriple_pure_preI\<close>.\<close>
+
+lemma cl_assn'_os_conv:
+  \<open>cl_assn' A xs p
+    = (EXS xsi. \<up>(length xsi = length xs) ** \<upharpoonleft>os_list_assn xsi p
+        ** \<upharpoonleft>(list_assn (mk_assn A)) xs xsi)\<close>
+  unfolding cl_assn'_def cl_assn_def olseg_def os_list_assn_def Proto_EOArray.list_assn_def
+  by (auto simp: sep_algebra_simps pred_lift_extract_simps fun_eq_iff)
+
+lemma htriple_pre_EXS:
+  assumes \<open>\<And>x. llvm_htriple (P x) c Q\<close>
+  shows \<open>llvm_htriple (EXS x. P x) c Q\<close>
+  apply (rule htripleI)
+  apply (clarsimp simp only: STATE_extract(3))
+  by (rule htripleD[OF assms])
+
+context begin
+
+private lemma cl_length_aux:
+  assumes B: \<open>length xs < max_snat LENGTH('l)\<close> and L: \<open>length xsi = length xs\<close>
+  shows \<open>llvm_htriple
+    (\<up>(length xsi = length xs) ** \<upharpoonleft>os_list_assn xsi p
+      ** \<upharpoonleft>(list_assn (mk_assn A)) xs xsi)
+    (cl_length p :: 'l::len2 word llM)
+    (\<lambda>n. \<upharpoonleft>snat.assn (length xs) n ** (EXS xsi'. \<up>(length xsi' = length xs)
+      ** \<upharpoonleft>os_list_assn xsi' p ** \<upharpoonleft>(list_assn (mk_assn A)) xs xsi'))\<close>
+proof -
+  have B': \<open>length xsi < max_snat LENGTH('l)\<close> using B L by simp
+  note H = frame_rule[OF cl_length_spine_rule[OF B'],
+    where F = \<open>\<upharpoonleft>(list_assn (mk_assn A)) xs xsi\<close>]
+  show ?thesis
+    apply (rule htriple_ent_pre[OF _ htriple_ent_post[OF _ H]])
+    subgoal
+      by (auto simp: entails_def sep_algebra_simps)
+    subgoal for n
+      apply (simp add: sep_conj_exists)
+      apply (rule entails_exI[where x = xsi])
+      by (auto simp: entails_def sep_algebra_simps L)
+    done
+qed
+
+lemma cl_length_rule[vcg_rules]:
+  \<open>length xs < max_snat LENGTH('l) \<Longrightarrow> llvm_htriple
+    (cl_assn' A xs p)
+    (cl_length p :: 'l::len2 word llM)
+    (\<lambda>n. \<upharpoonleft>snat.assn (length xs) n ** cl_assn' A xs p)\<close>
+  unfolding cl_assn'_os_conv
+  apply (rule htriple_pre_EXS)
+  subgoal for xsi
+    apply (rule htriple_pure_preI)
+    apply (rule cl_length_aux)
+     apply assumption
+    by (auto dest!: pure_part_split_conj)
+  done
+
+lemma cl_length_hnr[sepref_fr_rules]:
+  \<open>(cl_length, RETURN o op_list_length)
+  \<in> [\<lambda>xs. length xs < max_snat LENGTH('l::len2)]\<^sub>a (cl_assn' A)\<^sup>k \<rightarrow> (snat_assn' TYPE('l))\<close>
+  unfolding snat_rel_def snat.assn_is_rel[symmetric]
+  by (sepref_to_hoare; vcg)
+
+end
+
+text \<open>We define a generic list implementation and require the objects in our
+  list to implement a copy and a free function.
+  This copying setup is taken from
+  `isabelle_llvm/thys/examples/sorting/Sorting_Setup.thy`\<close>
+
+definition "is_copy A cp \<equiv> (cp, RETURN o COPY) \<in> A\<^sup>k \<rightarrow>\<^sub>a A"
+
+lemma is_copy_rule[sepref_fr_rules]:
+  "GEN_ALGO cp (is_copy A) \<Longrightarrow> (cp, RETURN o COPY) \<in> A\<^sup>k \<rightarrow>\<^sub>a A"
+  unfolding is_copy_def GEN_ALGO_def by auto
+
+lemma is_copy_pure_gen_algo: "CONSTRAINT is_pure A \<Longrightarrow> GEN_ALGO (Mreturn) (is_copy A)"  
+  unfolding is_copy_def GEN_ALGO_def
+  by (rule hnr_pure_COPY)
+
+locale copy_free_context =
+  fixes A :: \<open>'a \<Rightarrow> 'b::llvm_rep \<Rightarrow> assn\<close>
+    and afree_impl :: \<open>'b \<Rightarrow> unit llM\<close>
+    and acopy_impl :: \<open>'b \<Rightarrow> 'b llM\<close>
+  assumes a_assn_free[sepref_frame_free_rules]: \<open>MK_FREE A afree_impl\<close>
+  assumes a_assn_copy[sepref_gen_algo_rules]: \<open>GEN_ALGO acopy_impl (is_copy A)\<close>
+begin
+
+definition cl_copy :: \<open>'b cl_list \<Rightarrow> 'b cl_list llM\<close> where [llvm_code]:
+  \<open>cl_copy \<equiv> MMonad.REC (\<lambda>cl_copy p.
+    if p = null then Mreturn null else doM {
+      n \<leftarrow> ll_load p;
+      cpy \<leftarrow> acopy_impl (node.val n);
+      tl \<leftarrow> cl_copy (node.next n);
+      cl_prepend cpy tl
+    })\<close>
+
+end
+
+experiment begin
+
+definition \<open>nesttest xss = doN{
+  ASSERT(xss \<noteq> []);
+  ASSERT(hd xss \<noteq> []);
+  RETURN (hd (hd xss))
+}\<close> 
+
+end
+
+end
